AbstractStore.v
@@ -7,6 +7,14 @@ Definition abstract_store := total_map parity.
 Definition sound_store (ast : abstract_store) (st : store) : Prop := 
   forall x, gamma_par (ast x) (st x).
 
+Definition abstract_store_top : abstract_store :=
+  fun _ => par_top.
+Definition abstract_store_bottom : abstract_store :=
+  fun _ => par_bottom.
+Definition abstract_store_join
+    (ast1 ast2 : abstract_store) : abstract_store :=
+  fun x => parity_join (ast1 x) (ast2 x).
+
 Lemma t_update_sound : forall ast st x p n,
   sound_store ast st ->
   sound_par p n ->
